Program_Model.thy
@@ -2,18 +2,46 @@ theory Program_Model
   imports Statement_Semantics
 begin              
 
+
+section \<open>A\<close>
+
+text \<open>\<close>
+
 type_synonym program = \<open>(variables \<times> word \<times> var)\<close>
 
-locale bil =
-  fixes decode :: \<open>program \<Rightarrow> insn\<close>
 
-context bil
+section \<open>AAA\<close>
+
+locale bil =
+  fixes decode_pred :: \<open>program \<Rightarrow> insn \<Rightarrow> bool\<close> (infixr \<open>\<mapsto>\<^sub>b\<^sub>i\<^sub>r\<^sub>i\<close> 91) 
 begin
 
-definition
-  decode_pred :: \<open>program \<Rightarrow> insn \<Rightarrow> bool\<close> (\<open>_ \<mapsto>\<^sub>b\<^sub>i\<^sub>r\<^sub>i _\<close>)
+inductive
+  step_pred :: \<open>program \<Rightarrow> program \<Rightarrow> bool\<close> (infixr \<open>\<leadsto>\<^sub>b\<^sub>i\<^sub>l\<close> 90)
 where
-  \<open>(prog \<mapsto>\<^sub>b\<^sub>i\<^sub>r\<^sub>i instr) \<equiv> (instr = decode prog)\<close>
+  \<open>\<lbrakk>
+    ((\<Delta>, w, mem) \<mapsto>\<^sub>b\<^sub>i\<^sub>r\<^sub>i \<lparr> addr = w\<^sub>1, size = w\<^sub>2, code = bil \<rparr>); 
+    (\<Delta>, (w\<^sub>1 +\<^sub>b\<^sub>v w\<^sub>2) \<turnstile> bil \<leadsto> \<Delta>', w\<^sub>3, Empty)
+   \<rbrakk> \<Longrightarrow> ((\<Delta>, w, mem) \<leadsto>\<^sub>b\<^sub>i\<^sub>l (\<Delta>', w\<^sub>3, mem))\<close>
+
+lemma STEP: 
+  assumes \<open>(\<Delta>, w, mem) \<mapsto>\<^sub>b\<^sub>i\<^sub>r\<^sub>i \<lparr> addr = w\<^sub>1, size = w\<^sub>2, code = bil \<rparr>\<close>
+      and \<open>\<Delta>, (w\<^sub>1 +\<^sub>b\<^sub>v w\<^sub>2) \<turnstile> bil \<leadsto> \<Delta>', w\<^sub>3, Empty\<close>
+    shows \<open>(\<Delta>, w, mem) \<leadsto>\<^sub>b\<^sub>i\<^sub>l (\<Delta>', w\<^sub>3, mem)\<close>
+  using assms by (simp add: step_pred.intros)
+
+end 
+
+
+section \<open>AAA\<close>
+
+
+locale finite_bil = bil 
++  
+    fixes decode :: \<open>program \<Rightarrow> insn\<close>
+  assumes decode_pred_equiv: \<open>s \<mapsto>\<^sub>b\<^sub>i\<^sub>r\<^sub>i i \<longleftrightarrow> i = decode s\<close>
+      and decode_insn_finite: \<open>s \<mapsto>\<^sub>b\<^sub>i\<^sub>r\<^sub>i \<lparr> addr = w\<^sub>1, size = w\<^sub>2, code = bil \<rparr> \<Longrightarrow> bil_finite bil\<close>
+begin 
 
 fun
   step :: \<open>program \<Rightarrow> program\<close>
@@ -24,19 +52,14 @@ where
       (\<Delta>', w\<^sub>3, mem)
   )\<close>
 
-inductive (in bil)
-  step_pred :: \<open>program \<Rightarrow> program \<Rightarrow> bool\<close> (infixr \<open>\<leadsto>\<^sub>b\<^sub>i\<^sub>l\<close> 90)
-where
-  \<open>\<lbrakk>
-    (prog \<mapsto>\<^sub>b\<^sub>i\<^sub>r\<^sub>i \<lparr> addr = w\<^sub>1, size = w\<^sub>2, code = bil \<rparr>); 
-    (\<Delta>, (w\<^sub>1 +\<^sub>b\<^sub>v w\<^sub>2) \<turnstile> bil \<leadsto> \<Delta>', w\<^sub>3, Empty)
-   \<rbrakk> \<Longrightarrow> ((\<Delta>, w, mem) \<leadsto>\<^sub>b\<^sub>i\<^sub>l (\<Delta>', w', mem'))\<close>
+lemma \<open>(\<Delta>, w, mem) \<leadsto>\<^sub>b\<^sub>i\<^sub>l (\<Delta>', w', mem') \<Longrightarrow> (\<Delta>', w', mem') = step (\<Delta>, w, mem)\<close>
+  apply (induct rule: step_pred.inducts)
+  apply (drule_tac step_pred_bil_finite_empty)
+  using decode_insn_finite finite_bil_axioms apply blast
+  apply (simp add: decode_pred_equiv Let_def del: Bitvector_Syntax.add.simps)
+  by (metis old.prod.case select_convs(1) select_convs(2) select_convs(3))
 
-lemma STEP: 
-  assumes \<open>(\<Delta>, w, prog) \<mapsto>\<^sub>b\<^sub>i\<^sub>r\<^sub>i \<lparr> addr = w\<^sub>1, size = w\<^sub>2, code = bil \<rparr>\<close>
-      and \<open>\<Delta>, (w\<^sub>1 +\<^sub>b\<^sub>v w\<^sub>2) \<turnstile> bil \<leadsto> \<Delta>', w\<^sub>3, Empty\<close>
-    shows \<open>(\<Delta>, w, prog) \<leadsto>\<^sub>b\<^sub>i\<^sub>l (\<Delta>', w\<^sub>3, prog)\<close>
-  using assms by (simp add: step_pred.intros)
+end
 
-end 
+
 end
