BIR_64.thy
@@ -1,5 +1,5 @@
 theory BIR_64
-  imports BIR
+  imports BIR Word_Lib.Word_64
 begin
 
 definition 
